Add denotational semantics and some work on quadruples

Com.v
@@ -5,7 +5,7 @@ From Rela Require Import Bexp.
 Import BexpNotations.
 From Rela Require Import Proc.
 From Rela Require Import Sigma.
-From Coq Require Import Lia.
+
 From Coq Require Import Lists.List.
 
 Import ListNotations.
@@ -22,12 +22,12 @@ Definition variant : Type := sigma -> nat .
 
 Inductive com : Type :=
 | CSkip
-| CAss (x : Loc.t) (a: aexp)
+| CAssi (x : Loc.t) (a: aexp)
 | CAssr (x : Loc.t) (a : aexp)
 | CAssert (b: assertion )
 | CSeq (p1 : com) (p2 : com)
 | CIf (b : bexp) (p1 p2 : com)
-| CWhile (b : bexp) (p : com) (inv : assertion) (var : variant)
+| CWhile (b : bexp) (p : com) (inv : assertion) (var : variant) (id : nat)
 | CCall (f: Proc.t).
 
 (** Definition of procedure environment :
@@ -40,87 +40,6 @@ Module Psi.
   Definition empty_psi: psi := fun _ => CSkip.
 End Psi.
 
-(** Evaluation command as a relation **)
-
-Inductive ceval : com -> sigma -> Psi.psi -> sigma -> Prop :=
-  | E_Skip : forall s ps,
-      ceval CSkip s ps s
-  | E_Ass : forall s ps x a n,
-      aeval s a = n ->
-      ceval (CAss x a) s ps (x !-> n ; s)
-  | E_Assr : forall s ps x a n,
-      aeval s a = n ->
-      ceval (CAssr x a) s ps ((s x) !-> n ; s)
-  | E_Assert: forall s ps (b : assertion),
-      ceval (CAssert b) s ps s
-  | E_IfTrue : forall s s' ps b p1 p2,
-      beval s b = true ->
-      ceval p1 s ps s' ->
-      ceval (CIf b p1 p2) s ps s'
-  | E_IfFalse : forall s s' ps b p1 p2,
-      beval s b = false ->
-      ceval p2 s ps s' ->
-      ceval (CIf b p1 p2) s ps s'
-  | E_Seq : forall s s' s'' ps p1 p2,
-      ceval p1 s ps s' ->
-      ceval p2 s' ps s'' ->
-      ceval (CSeq p1 p2) s ps s''
-  | E_WhileFalse : forall b s ps p inv var,
-      beval s b = false ->
-      ceval (CWhile b p inv var) s  ps s
-  | E_WhileTrue : forall b s s' s'' ps p inv var,
-      beval s b = true ->
-      ceval p s ps s' ->
-      ceval (CWhile b p inv var) s' ps s'' ->
-      ceval (CWhile b p inv var) s  ps s''
-  | E_Call : forall s s' f ps,
-      ceval ( ps f) s ps s' ->
-      ceval (CCall f) s  ps s'
-.
-
-(** Facts about ceval **)
-
-Lemma ceval_inf_loop s ps s' inv var :
-ceval (CWhile BTrue CSkip inv var) s ps s' -> False.
-Proof.
-  intros Heval.
-  remember (CWhile BTrue CSkip inv var) as original_command eqn:Horig.
-  induction Heval;inversion Horig.
-  * inversion Horig;subst. inversion H.
-  * inversion Horig;subst.
-    apply IHHeval2. reflexivity.
-Qed.
-
-Lemma ceval_det s ps c:
-  forall s1' s2', ceval c s ps s1' -> ceval c s ps s2' -> s1' = s2'.
-Proof.
-  intros s1' s2' E1 E2.
-  generalize dependent s2'.
-  induction E1; intros st2' E2 ; inversion E2; subst.
-  - reflexivity.
-  - reflexivity.
-  - reflexivity.
-  - reflexivity.
-  - eapply IHE1; auto.
-  - rewrite H in H6.
-    discriminate H6.
-  - rewrite H in H6.
-    discriminate H6.
-  - eapply IHE1; auto.
-  - specialize (IHE1_1 s'0 H1).
-    subst.
-    apply (IHE1_2 _ H5).
-  - reflexivity.
-  - rewrite H in H7.
-    discriminate H7.
-  - rewrite H in H7.
-    discriminate H7.
-  - specialize (IHE1_1 s'0 H8).
-    subst.
-    apply (IHE1_2 _ H9).
-  - apply (IHE1 _ H0).
-Qed.
-
 (** Notations for program **)
 
 Declare Scope com_scope.
@@ -131,7 +50,7 @@ Module ComNotations.
 Notation "<[ e ]>" := (e) (e custom com at level 0) : com_scope.
 Notation "{ x }" := x (in custom com at level 0, x constr) : com_scope.
 Notation "'skip'" := (CSkip) (in custom com at level 1) : com_scope.
-Notation "x := y" := (CAss x y)
+Notation "x := y" := (CAssi x y)
             (in custom com at level 89,
              x custom aexp,
              y custom aexp,
@@ -151,11 +70,13 @@ Notation "'if' x 'then' y 'else' z 'end'" :=  (CIf x y z)
            x custom bexp at level 0,
            y custom com at level 0,
            z custom com at level 0) : com_scope.
-Notation "'while' x 'inv' i 'do' y 'end'" := (CWhile x y i)
+Notation "'while' x 'inv' i 'vari' v 'id' k 'do' y 'end'" := (CWhile x y i v k)
             (in custom com at level 89,
-            x custom bexp at level 0,
-            y custom com at level 0,
-            i constr at level 0) : com_scope.
+             x custom bexp at level 0,
+             y custom com at level 0,
+             i constr at level 0,
+             v constr at level 0,
+             k constr at level 0) : com_scope.
 Notation "'call' f" := (CCall f)
             (in custom com at level 89,
             f constr at level 0) : com_scope.
