Sem.v
@@ -1,0 +1,461 @@
+From Rela Require Import Loc.
+From Rela Require Import Aexp.
+Import AexpNotations.
+From Rela Require Import Bexp.
+Import BexpNotations.
+From Rela Require Import Proc.
+From Rela Require Import Sigma.
+From Rela Require Import Com.
+From Rela Require Import function_cpo constructs.
+
+(** Evaluation command as a relation **)
+
+Inductive ceval : com -> sigma -> Psi.psi -> sigma -> Prop :=
+  | E_Skip : forall s ps,
+      ceval CSkip s ps s
+  | E_Assi : forall s ps x a n,
+      aeval s a = n ->
+      ceval (CAssi x a) s ps (x !-> n ; s)
+  | E_Assr : forall s ps x a n,
+      aeval s a = n ->
+      ceval (CAssr x a) s ps ((s x) !-> n ; s)
+  | E_Assert: forall s ps (b : assertion),
+      ceval (CAssert b) s ps s
+  | E_IfTrue : forall s s' ps b p1 p2,
+      beval s b = true ->
+      ceval p1 s ps s' ->
+      ceval (CIf b p1 p2) s ps s'
+  | E_IfFalse : forall s s' ps b p1 p2,
+      beval s b = false ->
+      ceval p2 s ps s' ->
+      ceval (CIf b p1 p2) s ps s'
+  | E_Seq : forall s s' s'' ps p1 p2,
+      ceval p1 s ps s' ->
+      ceval p2 s' ps s'' ->
+      ceval (CSeq p1 p2) s ps s''
+  | E_WhileFalse : forall b s ps p inv var id,
+      beval s b = false ->
+      ceval (CWhile b p inv var id) s  ps s
+  | E_WhileTrue : forall b s s' s'' ps p inv var id,
+      beval s b = true ->
+      ceval p s ps s' ->
+      ceval (CWhile b p inv var id) s' ps s'' ->
+      ceval (CWhile b p inv var id) s  ps s''
+  | E_Call : forall s s' f ps,
+      ceval ( ps f) s ps s' ->
+      ceval (CCall f) s  ps s'
+.
+
+(** Facts about ceval **)
+
+Lemma ceval_inf_loop s ps s' inv var id:
+ceval (CWhile BTrue CSkip inv var id) s ps s' -> False.
+Proof.
+  intros Heval.
+  remember (CWhile BTrue CSkip inv var id) as original_command eqn:Horig.
+  induction Heval;inversion Horig.
+  * inversion Horig;subst. inversion H.
+  * inversion Horig;subst.
+    apply IHHeval2. reflexivity.
+Qed.
+
+Lemma ceval_det s ps c:
+  forall s1' s2', ceval c s ps s1' -> ceval c s ps s2' -> s1' = s2'.
+Proof.
+  intros s1' s2' E1 E2.
+  generalize dependent s2'.
+  induction E1; intros st2' E2 ; inversion E2; subst.
+  - reflexivity.
+  - reflexivity.
+  - reflexivity.
+  - reflexivity.
+  - eapply IHE1; auto.
+  - rewrite H in H6.
+    discriminate H6.
+  - rewrite H in H6.
+    discriminate H6.
+  - eapply IHE1; auto.
+  - specialize (IHE1_1 s'0 H1).
+    subst.
+    apply (IHE1_2 _ H5).
+  - reflexivity.
+  - rewrite H in H8.
+    discriminate H8.
+  - rewrite H in H8.
+    discriminate H8.
+  - specialize (IHE1_1 s'0 H9).
+    subst.
+    apply (IHE1_2 _ H10).
+  - apply (IHE1 _ H0).
+Qed.
+
+(** Evaluation command as a function **)
+
+(* https://github.com/rocq-community/semantics *)
+
+Definition bind (A B:Type)(v:option A)(f:A->option B) : option B :=
+  match v with Some x => f x | None => None end.
+
+Arguments bind : default implicits.
+
+(*This proof can more modular, the sale for W_phi_continuous *)
+
+Lemma bind_continuous :
+  forall (A B:Type) F G,
+    continuous (f_order A B) (f_order' B) F ->
+    continuous (f_order A B) (f_order' B) G ->
+    continuous (f_order A B) (f_order' B)
+      (fun f x => bind (F f x) (G f)).
+Proof.
+  unfold f_order'.
+  intros A B F G HFc HGc c Hc l H.
+  specialize (HFc c Hc l H) as HF.
+  specialize (HGc c Hc l H) as HG.
+  clear H.
+  apply lift_lub.
+  intros x.
+  split.
+  - intros n.
+    destruct HF as [HF _].
+    specialize (HF n x); simpl in HF.
+    inversion HF;[auto |].
+    destruct x0;rewrite <- H;[simpl|auto].
+    destruct HG as [HG _].
+    specialize (HG n b);simpl in HG.
+    inversion HG;auto.
+  - intros y Hu.
+    case_eq (F l x);[|auto].
+    + intros x0 H; simpl.
+      specialize (lub_some_witness _ _ _ _ _ _ H HF) as [nf Hf].
+      case_eq (G l x0);[|auto].
+      * intros ? H0; simpl.
+        specialize (lub_some_witness _ _ _ _ _ _ H0 HG) as [ng Hg].
+        specialize (Hu (nf + ng)); simpl in Hu.
+        specialize
+          (transitive_lift A _ (@option_cpo B) (transitive_option_cpo B))
+          as Htc.
+        specialize
+          (reflexive_lift A _ (@option_cpo B) (reflexive_option_cpo B))
+          as Hrc.
+        generalize (chain_le _ _ Htc Hrc _ _ _ Hc (Nat.le_add_r nf ng)).
+        specialize (continuous_imp_monotonic _ _ _ _ F Hrc HFc) as HFm.
+        intros HFcc %(HFm _ _).
+        specialize (HFcc x).
+        rewrite Hf in HFcc.
+        inversion HFcc; subst.
+        rewrite <- H3 in Hu; simpl in Hu.
+        generalize (chain_le _ _ Htc Hrc c _ _ Hc (Nat.le_add_l ng nf)).
+        specialize (continuous_imp_monotonic _ _ _ _ G Hrc HGc) as HGm.
+        intros HGcc %(HGm _ _).
+        specialize (HGcc x0).
+        rewrite Hg in HGcc.
+        inversion HGcc;subst.
+        rewrite <- H4 in Hu.
+        assumption.
+Qed.
+
+Module W_phi.
+
+  Definition F_phi (A:Type)(t:A->option bool)(f g :A->option A) :=
+    fun r => 'IF (t r) 'THEN (bind (f r) g) 'ELSE (Some r).
+
+  Theorem F_phi_continuous :
+    forall (A : Type) t f,
+      continuous (f_order A A)(f_order A A) (F_phi A t f).
+  Proof.
+    intros A t f; unfold F_phi.
+      apply ifthenelse_continuous with (F:= comp_right f)
+                                       (G:= fun (g:A->option A)(x:A) => Some x).
+    apply comp_right_continuous.
+    apply continuous_cst; auto.
+  Qed.
+
+  Definition phi := fun A t f => Tarski_fix (F_phi A t f).
+
+  Arguments phi : default implicits.
+
+  Lemma phi_terminates_n :
+    forall (A:Type) (t:A->option bool)  f r r',
+      phi t f r = Some r' ->
+      exists n, iter _ (F_phi A t f) n (fun g => None) r = Some r'.
+  Proof.
+    intros A t f r r' Heq.
+    assert (Hlub : lub (f_order' A) (phi t f)
+                     (fun n => iter _ (F_phi A t f) n (fun x : A => None))).
+    apply least_fixpoint_lub_iterates; auto.
+    intros g x; apply option_cpo_none_bot.
+    unfold f_order'; apply F_phi_continuous.
+    unfold phi, F_phi, f_order'; apply Tarski_fix_prop.
+    exact (F_phi_continuous A t f).
+    apply (lub_some_witness _ _ _ r r' (phi t f) Heq Hlub).
+  Qed.
+
+  Lemma fix_phi :
+    forall (A:Type)(t:A->option bool) f,
+      F_phi A t f (phi t f) = phi t f.
+  Proof.
+    intros A t f.
+    assert (Hint : least_fixpoint (f_order' A) (F_phi A t f) (phi t f)).
+    unfold phi, f_order'; apply Tarski_fix_prop; apply F_phi_continuous.
+    unfold least_fixpoint in Hint; fold (phi t f) in Hint.
+    intuition.
+  Qed.
+
+  Lemma always_witness A B:
+    forall (F : (A -> option B) -> B -> option B)
+      (c : nat -> A -> option B)
+      (l : A -> option B),
+      lub (f_order' B) (F l) (fun n : nat => F (c n)) ->
+      forall x, exists n, @option_cpo B (F l x) (F (c n) x).
+  Proof.
+    intros F c l HF x.
+    specialize (lub_lift_reverse _ _ _ _ _ HF) as HF'.
+    simpl in HF'.
+    case_eq (F l x).
+    - intros b Hb.
+      specialize (HF' x).
+      rewrite Hb in HF'.
+      specialize (lub_some_witness1 _ _ _ HF') as [w Hw].
+      exists w. rewrite Hw. auto.
+    - intros. exists 0. auto.
+  Qed.
+
+  Lemma iter_phi :
+    forall (A B : Type)
+      F
+      (t : B -> option bool)
+      (c : nat -> A -> option B)
+      w b n x,
+      iter (B -> option B) (F_phi B t (F (c n))) w (fun _ : B => None) x = Some b ->
+      W_phi.phi t (F (c n)) x = Some b.
+  Proof.
+    intros ?? F t c w ? ?.
+    induction w.
+    - intros ? Hw; inversion Hw.
+    - simpl; intros x.
+      rewrite <- W_phi.fix_phi.
+      unfold W_phi.F_phi at 1 3.
+      case (t x);[| discriminate ].
+      intros b0;case b0;[simpl|auto].
+      case_eq (F (c n) x);[simpl| intros ? Hb; inversion Hb].
+      intros x' Hx' Hn.
+      apply IHw.
+      assumption.
+  Qed.
+
+  Theorem W_phi_continuous :
+    forall (A B:Type) F t,
+      continuous (f_order A B) (f_order' B) F ->
+      continuous (f_order A B) (f_order' B)
+        (fun f x => W_phi.phi t (F f) x).
+  Proof.
+    intros A B F t HFc c Hc l Hl.
+    specialize (HFc c Hc l Hl) as HF.
+    apply lift_lub.
+    intros x.
+    split.
+    - intros n.
+      case_eq (W_phi.phi t (F (c n)) x);[|auto].
+      intros b [nb <-] %(W_phi.phi_terminates_n _ _ _ _ _).
+      revert x.
+      induction nb ;[auto |].
+      simpl;intros x.
+      rewrite <- W_phi.fix_phi.
+      unfold W_phi.F_phi at 1 3.
+      case (t x);[|auto]; intros b0.
+      case b0;simpl;[|auto].
+      destruct HF as [HF _].
+      specialize (HF n x);simpl in HF.
+      inversion HF;[auto |].
+      rewrite <- H.
+      case x0;[|auto].
+      simpl.
+      apply IHnb.
+    - intros y Hy.
+      specialize (always_witness _ _ _ _ _ HF) as Hx.
+      case_eq (W_phi.phi t (F l) x);[|auto].
+      intros b Hb.
+      specialize (W_phi.phi_terminates_n _ _ _ _ _ Hb) as [w Hw].
+      assert (truc : exists n,
+                 iter (B -> option B) (W_phi.F_phi B t (F (c n))) w (fun _ : B => None) x
+                 = Some b).
+      { clear Hy Hb.
+        generalize dependent x.
+        induction w.
+        - intros x Hw; inversion Hw.
+        - intros x; simpl.
+          unfold W_phi.F_phi at 1 3.
+          case (t x);[|discriminate].
+          intros b0;case b0;[simpl|exists 0;auto].
+          simpl.
+          case_eq (F l x);[simpl| discriminate].
+          intros x' Hx' [n Hn] %(IHw _).
+          specialize (Hx x) as [n' Hn'].
+          rewrite Hx' in Hn'.
+          inversion Hn'.
+          exists (n' + n).
+          specialize
+            (transitive_lift A _ (@option_cpo B) (transitive_option_cpo B))
+            as Htc.
+          specialize
+            (reflexive_lift A _ (@option_cpo B) (reflexive_option_cpo B))
+            as Hrc.
+          generalize (chain_le _ _ Htc Hrc _ _ _ Hc (Nat.le_add_r n' n)).
+          specialize (continuous_imp_monotonic _ _ _ _ F Hrc HFc) as HFm.
+          intros HFcc %(HFm _ _).
+          specialize (HFcc x).
+          rewrite <- H1 in HFcc.
+          inversion HFcc.
+          simpl.
+          revert Hn. revert Htc. revert Hrc. revert Hc. revert HFc. clear.
+          intros HFc Hc Hrc Htc.
+          revert x'.
+          induction w.
+          + intros ? Hn;inversion Hn.
+          + simpl. intros x.
+            unfold W_phi.F_phi at 1 3.
+            case (t x);[|eauto].
+            intros b0;case b0;[simpl|auto].
+            case_eq (F (c n) x);[simpl| discriminate ].
+            intros x' Hx' Hn.
+            generalize (chain_le _ _ Htc Hrc _ _ _ Hc (Nat.le_add_l n n')).
+            specialize (continuous_imp_monotonic _ _ _ _ F Hrc HFc) as HFm.
+            intros HFcc %(HFm _ _).
+            specialize (HFcc x).
+            rewrite Hx' in HFcc.
+            inversion HFcc.
+            simpl.
+            apply IHw.
+            assumption.
+      }
+      destruct truc.
+      specialize (Hy x0).
+      simpl in Hy.
+      apply iter_phi in H.
+      rewrite H in Hy.
+      assumption.
+  Qed.
+
+End W_phi.
+
+Module Psi'.
+  Definition psi : Type := (Proc.t * sigma) -> option sigma.
+
+  Definition empty_psi: psi := fun x => Some (snd x).
+End Psi'.
+
+Fixpoint ds  (ps : Psi'.psi) (i : com) : sigma -> option sigma :=
+  match i with
+  | CSkip => fun r => Some r
+  | CAssi x a => fun l => bind (Some (aeval l a)) (fun v => Some (x !-> v; l))
+  | CAssr x a => fun l => bind (Some (aeval l a)) (fun v => Some ((l x) !-> v; l))
+  | CAssert a => fun r => Some r
+  | CSeq i1 i2 => fun r => bind (ds ps i1 r) (ds ps i2)
+  | CIf b i1 i2 => fun l => if beval l b then ds ps i1 l else ds ps i2 l
+  | CWhile b p inv var id => fun l => W_phi.phi (fun l' => Some (beval l' b)) (ds ps p) l
+  | CCall f => fun l => ps (f, l)
+  end.
+
+Module F_phi.
+
+  Lemma ds_continuous :
+    forall i,
+      continuous
+        (f_order (Proc.t * sigma) sigma)
+        (f_order sigma sigma)
+        (fun ps => ds ps i).
+  Proof.
+    induction i.
+    - intros c  _ ps _;  simpl.
+      apply lub_cst.
+      apply reflexive_f_order.
+    - intros c  _ ps _;  simpl.
+      apply lub_cst.
+      apply reflexive_f_order.
+    - intros c  _ ps _;  simpl.
+      apply lub_cst.
+      apply reflexive_f_order.
+    - intros c  _ ps _;  simpl.
+      apply lub_cst.
+      apply reflexive_f_order.
+    - simpl; apply bind_continuous; assumption.
+    - simpl.
+      apply
+        (ifthenelse_continuous
+           (Proc.t * sigma) sigma (fun x => Some (beval x b)) _ _ IHi1 IHi2).
+    - simpl; apply W_phi.W_phi_continuous; assumption.
+    - simpl. intros c Hc l Hl.
+      split.
+      * intros n s.
+        destruct Hl as [Hl _].
+        specialize (Hl n (f,s)).
+        assumption.
+      * intros y Hy s.
+        case_eq (l (f,s));[|auto].
+        intros x H.
+        specialize (lub_some_witness _ _ _ _ _ _ H Hl) as [n Hx].
+        specialize (Hy n s);simpl in Hy.
+        rewrite <- Hx.
+        assumption.
+  Qed.
+
+  Definition F_phi ps (ps' : Psi'.psi) : Psi'.psi :=
+    fun x => ds ps' (ps (fst x)) (snd x).
+
+  Theorem F_phi_continuous :
+    forall ps,
+      continuous
+        (f_order (Proc.t * sigma) sigma)
+        (f_order (Proc.t * sigma) sigma) (F_phi ps).
+  Proof.
+    intros ps c Hc l [Hu Hl].
+    unfold F_phi.
+    split.
+    - intros n [p s];  simpl.
+      specialize (ds_continuous (ps p) c Hc l (conj Hu Hl)) as [Hu' _].
+      apply Hu'.
+    - intros ds' Hds' [ p s]; simpl.
+      specialize (ds_continuous (ps p) c Hc l (conj Hu Hl)) as [_ Hl'].
+      apply (Hl' (fun s => ds' (p,s))).
+      intros n s'.
+      apply (Hds' n (p,s')).
+  Qed.
+
+  Definition phi := fun ps => Tarski_fix (F_phi ps).
+
+  Arguments phi : default implicits.
+
+  Lemma phi_terminates_n :
+    forall ps r r',
+      phi ps r = Some r' ->
+      exists n, iter _ (F_phi ps) n (fun _ => None) r = Some r'.
+    intros ps r r' Heq.
+    apply (lub_some_witness _ _
+                (fun n => iter _ (F_phi ps) n (fun _ => None)) r r' (phi ps) Heq).
+    apply least_fixpoint_lub_iterates.
+    + unfold reflexive.
+      unfold lift_order.
+      intros; apply option_cpo_refl.
+    + apply antisymmetric_lift.
+      apply antisym_option_cpo.
+    + apply lift_complete.
+      apply complete_option_cpo.
+    + intros x g; apply option_cpo_none_bot.
+    + apply F_phi_continuous.
+    + unfold phi, F_phi, f_order'; apply Tarski_fix_prop.
+      exact (F_phi_continuous ps).
+  Qed.
+
+  Lemma fix_phi :
+    forall ps, F_phi ps (phi ps) = phi ps.
+  Proof.
+    intros ps.
+    assert (Hint : least_fixpoint (f_order (Proc.t * sigma) sigma) (F_phi ps) (phi ps)).
+    unfold phi, f_order'; apply Tarski_fix_prop; apply F_phi_continuous.
+    unfold least_fixpoint in Hint; fold (phi ps) in Hint.
+    intuition.
+  Qed.
+
+End F_phi.
+
+Definition denot c s ps := ds (F_phi.phi ps) c s.
