Sem_Prop.v
@@ -1,0 +1,94 @@
+From Rela Require Import Loc.
+From Rela Require Import Aexp.
+Import AexpNotations.
+From Rela Require Import Bexp.
+Import BexpNotations.
+From Rela Require Import Proc.
+From Rela Require Import Sigma.
+From Rela Require Import Com.
+From Rela Require Import Sem.
+From Rela Require Import Inliner.
+From Rela Require Import function_cpo constructs.
+
+Theorem ds_sn :  forall i l l' ps, denot i l ps = Some l' -> ceval i l ps l'.
+  induction i.
+  - unfold denot, ds.
+    injection 1 as ->.
+    apply E_Skip.
+  - unfold denot, ds, bind.
+    injection 1 as <-.
+    now apply E_Assi.
+  - unfold denot, ds, bind.
+    injection 1 as <-.
+    now apply E_Assr.
+  - unfold denot, ds, bind.
+    injection 1 as <-.
+    now apply E_Assert.
+  - intros l l' ps; unfold denot; simpl; unfold bind.
+    case_eq (ds (F_phi.phi ps) i1 l); intros s' Hs'.
+    + intros; apply (E_Seq _ s'); [now apply IHi1| now apply IHi2].
+    + discriminate Hs'.
+  - intros l l' ps; unfold denot; simpl.
+    case_eq (beval l b); intros Hb H.
+    + apply E_IfTrue; [assumption | now apply IHi1].
+    + apply E_IfFalse; [assumption | now apply IHi2].
+  - intros l l' ps H.
+    pose (f:= W_phi.F_phi _ (fun l => Some (beval l b)) (ds (F_phi.phi ps) i)).
+    assert (Hn: exists n:nat,
+               iter _ f n (fun _ : sigma => None) l = Some l').
+    { apply W_phi.phi_terminates_n. assumption. }
+    destruct Hn as [n Hn].
+    clear H; generalize dependent l.
+    induction n;simpl;intros l.
+    + discriminate.
+    + unfold f at 1, W_phi.F_phi , ifthenelse at 1.
+      case_eq (beval l b);intros Hb.
+      * unfold bind.
+        case_eq (ds (F_phi.phi ps) i l);intros.
+        -- now apply (E_WhileTrue _ _ s);[|apply IHi |apply IHn].
+        -- discriminate.
+      * injection 1 as <-.
+        now apply E_WhileFalse.
+  - intros l l' ps H.
+    apply F_phi.phi_terminates_n in H.
+    destruct H as [n Hn].
+    assert(H: ds (iter Psi'.psi (F_phi.F_phi ps) n (fun _ : Proc.t * sigma => None)) (CCall f) l = Some l');
+    [apply Hn | clear Hn].
+    apply Inline2.ds_iter_ds_k_inliner in H.
+    apply Inline2.ds_none_ceval_none in H.
+    apply Inline1.inline_n_ceval with (S n).
+    now apply Inline2.ceval_inline2_inline1.
+Qed.
+
+Theorem sn_ds : forall l i l' ps , ceval i l ps l' -> denot i l ps = Some l'.
+  induction 1.
+  - auto.
+  - rewrite <- H. reflexivity.
+  - rewrite <- H; reflexivity.
+  - reflexivity.
+  - unfold denot. simpl.
+    rewrite H. assumption.
+  - unfold denot. simpl.
+    rewrite H. assumption.
+  - unfold denot. simpl.
+    unfold denot in IHceval1.
+    rewrite IHceval1.  assumption.
+  - unfold denot. simpl.
+    rewrite <- W_phi.fix_phi.
+    unfold W_phi.F_phi.
+    rewrite H. reflexivity.
+  - unfold denot. simpl.
+    rewrite <- W_phi.fix_phi.
+    unfold W_phi.F_phi.
+    rewrite H. simpl.
+    unfold denot in IHceval1.
+    rewrite IHceval1. assumption.
+  - unfold denot. simpl.
+    rewrite <- F_phi.fix_phi.
+    unfold F_phi.F_phi.
+    assumption.
+Qed.
+
+Theorem ds_eq_sn : forall i l l' ps, denot i l ps = Some l' <-> ceval i l ps l'.
+intros; split; [apply ds_sn | apply sn_ds]; auto.
+Qed.
