Vcg_Quadruple.v
@@ -1,0 +1,214 @@
+From Rela Require Import Vcg.
+From Rela Require Import Bexp.
+From Rela Require Import Com.
+From Rela Require Import Sem.
+From Rela Require Import Sigma.
+From Rela Require Import Hoare_Triple.
+From Rela Require Import Quadruple.
+From Rela Require Import Vcg_Rela.
+
+From Coq Require Import Lists.List.
+Import ListNotations.
+
+(** Defintion of the verification condition generator for quadruples,
+    using the verification condition generator for relational properties **)
+
+Definition q_suite : Type := Sigma.sigma -> Sigma.sigma -> history ->  history -> Prop.
+
+Definition to_rsuite (suite: q_suite) : r_suite :=
+  fun ml hl => match ml, hl with
+            | m1 :: m2 :: [], h1 :: h2 :: [] => suite m1 m2 h1 h2
+            | _, _ => False
+            end.
+
+Definition qtc (c1 c2: com) (m1 m2: Sigma.sigma) (h1 h2: history)
+  (cls: Phi.phi) (suite: q_suite) : Prop :=
+  let cl := c1 :: [c2] in
+  let ml := m1 :: [m2] in
+  let hl := h1 :: [h2] in
+  rtc cl ml hl cls (to_rsuite suite) eq_refl eq_refl.
+
+(** Defintion of the generator of auxiliare goals for relational quadruples **)
+
+Definition qtc' (c1 c2: com) (m1 m2: Sigma.sigma) (h1 h2: history)
+  (cls: Phi.phi): Prop :=
+  let cl := c1 :: [c2] in
+  let ml := m1 :: [m2] in
+  let hl := h1 :: [h2] in
+  rtc' cl ml hl cls eq_refl eq_refl.
+
+(** Defintion of the verification condition generator for quadruple on loop **)
+
+Definition qwtc (c1 c2 : com) (h1 h2: history)
+  (cls: Phi.phi) (inv : q_assertion) (L R : q_cond) b1 b2: Prop :=
+  (forall m1 m2,
+      inv m1 m2 -> Assn_b.bassn b1 m1 -> Assn_b.bassn b2 m2 ->
+      L m1 m2 = false -> R m1 m2 = false ->
+      (qtc' c1 c2 m1 m2 h1 h2 cls /\
+         qtc c1 c2 m1 m2 h1 h2 cls (fun m1' m2' _ _ =>  inv m1' m2')))
+  /\
+    (forall m1 m2,
+        inv m1 m2 -> Assn_b.bassn b1 m1 -> L m1 m2 = true  ->
+        (qtc' c1 CSkip m1 m2 h1 h2 cls /\
+           qtc c1 CSkip m1 m2 h1 h2 cls (fun m1' m2' _ _ =>  inv m1' m2')))
+  /\
+    (forall m1 m2,
+        inv m1 m2-> Assn_b.bassn b2 m2 -> R m1 m2 = true ->
+        (qtc' CSkip c2 m1 m2 h1 h2 cls /\
+           qtc CSkip c2 m1 m2 h1 h2 cls (fun m1' m2' _ _ =>  inv m1' m2')))
+  /\
+    (forall m1 m2, inv m1 m2 ->
+              beval m1 b1 = beval m2 b2 \/
+                (beval m1 b1 = true /\ L m1 m2 = true ) \/
+                (beval m2 b2 = true /\ R m1 m2 = true)).
+
+(** Translation of a quadruple on loop into Prop **)
+
+Definition while_call b p inv var ps s s' id :=
+  ceval (CWhile b p inv var id) s ps s'.
+
+Definition twq (qwl: QW_Phi.phi) ps :=
+  forall c1 c2 b1 b2 inv1 inv2 var1 var2 s1 s1' s2 s2' n1 n2,
+    while_call b1 c1 inv1 var1 ps s1 s1' n1 ->
+    while_call b2 c2 inv2 var2 ps s2 s2' n2 ->
+    get_wq_inv (qwl c1 b1 n1 c2 b2 n2 ) s1 s2 ->
+    get_wq_inv (qwl c1 b1 n1 c2 b2 n2 ) s1' s2' /\
+      beval s1' b1 = false /\ beval s2' b2 = false.
+
+Lemma tr_quadruple_while (qwl: QW_Phi.phi) ps :
+  (forall inv1 inv2 var1 var2 c1 c2 b1 b2 id1 id2,
+      let wq_clause := qwl c1 b1 id1 c2 b2 id2 in
+      let q_inv := get_wq_inv wq_clause in
+      quadruple q_inv
+        (fun m1 m2  _ _ => q_inv m1 m2 /\
+                          beval m1 b1 = false /\ beval m2 b2 = false)
+        (CWhile b1 c1 inv1 var1 id1)
+        (CWhile b2 c2 inv2 var2 id2) ps)
+  -> twq qwl ps.
+Proof.
+intros H c1 c2 b1 b2 inv1 inv2 var1 var2 s1 s1' s2 s2' id1 id2 hw1 hw2 hinv.
+eapply H;eauto.
+Qed.
+
+(** Adding while_call to invariant of while **)
+
+Definition mk_while_call b p inv var ps id h :=
+  match h with
+  | s :: (s' :: _) => while_call b p inv var ps s s' id
+  | _ => False
+  end.
+
+Fixpoint inv_call c ps : com :=
+    match c with
+    | CSkip => c
+    | CAssi x a => c
+    | CAssr x a => c
+    | CAssert b => c
+    | CSeq p1 p2 => CSeq (inv_call p1 ps) (inv_call p2 ps)
+    | CIf b p1 p2 => CIf b (inv_call p1 ps) (inv_call p2 ps)
+    | CWhile b p inv var id =>
+        CWhile b (inv_call p ps)
+          (fun h => inv h /\ mk_while_call b p inv var ps id h)
+          var id
+    | CCall f => c
+    end.
+
+Lemma inv_call_ceval c ps:
+forall s s', ceval (inv_call c ps) s ps s' <->  ceval c s ps s'.
+Proof.
+  induction c; intros.
+  all: split; intros; auto.
+  1-2: inversion H;subst;
+       eapply E_Seq;[ apply IHc1| apply IHc2]; eauto.
+  1-2: inversion H;subst;
+      [ apply E_IfTrue;[auto|apply IHc1;auto] |
+        apply E_IfFalse;[auto|apply IHc2;auto]].
+  - remember (CWhile b c inv var id) as original_command eqn:Horig.
+    remember (inv_call original_command ps) as original_command2 eqn:Horig2.
+    induction H; subst; inversion Horig2;subst.
+      + eapply E_WhileFalse; assumption.
+      + eapply E_WhileTrue;[assumption | apply IHc;eauto|auto].
+  - remember (CWhile b c inv var id) as original_command eqn:Horig.
+    remember (inv_call original_command ps) as original_command2 eqn:Horig2.
+    induction H; subst; inversion Horig;subst.
+      + eapply E_WhileFalse; assumption.
+      + eapply E_WhileTrue;[assumption | apply IHc;eauto|auto].
+Qed.
+
+(* Lemma inv_call_hoare : *)
+(*   forall (inv: assertion) (var: variant) b c ps l id si, *)
+(*     hoare_triple (fun s => inv (s :: (si :: l))) *)
+(*       (fun s' _ => inv (s' :: (si :: l)) /\ beval s'  b = false) *)
+(*       (CWhile b c inv var id) ps -> *)
+(*     hoare_triple (fun s => inv (s :: (si :: l))) *)
+(*       (fun s' _ => inv (s' :: (si :: l)) /\ beval s'  b = false) *)
+(*       (inv_call (CWhile b c inv var id) ps) ps. *)
+(* Proof. *)
+(*   intros. *)
+(*   intros s s' HPre Heval. *)
+(*   eapply H;[apply HPre | apply inv_call_ceval;auto]. *)
+(* Qed. *)
+
+(** Definition of a verification condition generator for quadruple on procedures **)
+
+Definition qtr (qcl: Q_Phi.phi) (ps: Psi.psi) :=
+  forall p1 p2 s1 s2 s1' s2',
+    proc_to_pred (p1 :: [p2]) (s1 :: [s2]) (s1' :: [s2']) ps eq_refl eq_refl ->
+    (get_q_pre (qcl p1 p2)) s1 s2 -> (get_q_post (qcl p1 p2)) s1' s2' s1 s2.
+
+(** Facts about tr **)
+
+Lemma qtr_relational_prop (qcl:Q_Phi.phi) (ps: Psi.psi):
+  (forall p1 p2,
+      quadruple
+        (get_q_pre (qcl p1 p2))
+        (get_q_post (qcl p1 p2))
+        (CCall p1)  (CCall p2)ps)
+  -> qtr qcl ps.
+Proof.
+  intros H  p1 p2 s1 s2 s1' s2' Hcall Hp.
+  apply rceval_proc_to_prod in Hcall.
+  inversion Hcall;subst.
+  inversion H8;subst.
+  apply H;auto.
+Qed.
+
+(** Definition of a verification condition generator for quadruple on procedures **)
+
+Definition qtc_p (ps: Psi.psi) (cls: Phi.phi) (qcl: Q_Phi.phi): Prop :=
+  forall f1 f2 ps',
+    let c1 := ps f1 in
+    let c2 := ps f2 in
+    (forall m1 m2,
+        get_q_pre (qcl f1 f2) m1 m2 /\
+          qtr qcl ps' /\
+          get_LR(qcl f1 f2) m1 m2 = true /\
+          get_L(qcl f1 f2) m1 m2 = false /\
+          get_R(qcl f1 f2) m1 m2 = false ->
+        (qtc' c1 c2 m1 m2 empty_history empty_history (phi_call cls ps') /\
+           qtc c1 c2  m1 m2 empty_history empty_history (phi_call cls ps')
+             (fun m1' m2' _ _ => (get_q_post (qcl f1 f2)) m1' m2' m1 m2)))
+    /\
+    (forall m1 m2,
+        get_q_pre (qcl f1 f2) m1 m2 /\
+          qtr qcl ps' /\
+          get_L(qcl f1 f2) m1 m2 = true ->
+        (qtc' c1 CSkip m1 m2 empty_history empty_history (phi_call cls ps') /\
+           qtc c1 CSkip  m1 m2 empty_history empty_history (phi_call cls ps')
+             (fun m1' m2' _ _ => (get_q_post (qcl f1 f2)) m1' m2' m1 m2))) /\
+    (forall m1 m2,
+        get_q_pre (qcl f1 f2) m1 m2 /\
+          qtr qcl ps' /\
+          get_R(qcl f1 f2) m1 m2 = true ->
+        (qtc' CSkip c2 m1 m2 empty_history empty_history (phi_call cls ps') /\
+           qtc CSkip c2 m1 m2 empty_history empty_history (phi_call cls ps')
+             (fun m1' m2' _ _ => (get_q_post (qcl f1 f2)) m1' m2' m1 m2)))
+      /\
+        (forall m1 m2,  get_q_pre (qcl f1 f2) m1 m2 ->
+                   ((get_LR(qcl f1 f2) m1 m2 = true /\
+                       get_L(qcl f1 f2) m1 m2 = false /\
+                       get_R(qcl f1 f2) m1 m2 = false)
+                    \/
+                      get_L(qcl f1 f2) m1 m2 = true
+                    \/
+                      get_R(qcl f1 f2) m1 m2 = true)).
